src/Data/TwoThreeTreesWF.v
@@ -12,6 +12,7 @@ Require Import FP.Structures.Eqv.
 Require Import FP.Structures.Additive.
 Require Import FP.Relations.RelDec.
 
+Import EqvNotation.
 Import OrdNotation.
 Import AdditiveNotation.
 
@@ -20,11 +21,53 @@ Module TwoThreeTreesWF.
 
   Section Context.
     Context {K:Type}.
-    Context {E:Eqv K}.
+    Context {E:Eqv K} {EWF:EqvWF K}.
     Context {O:Ord K} {OWF:OrdWF K}.
-    Context {L:Lattice K} {B:BoundedLattice K}.
+    Context {L:Lattice K} {LWF:LatticeWF K}.
+    Context {B:BoundedLattice K} {BWF:BoundedLatticeWF K}.
     Context {OD:OrdDec K} {ODC:OrdDecCorrect K}.
     Context {V:Type}.
+
+    Inductive in_tree : K -> tree K V -> Prop :=
+      | InTwoLeftTree :
+          forall k tl pm tr,
+            in_tree k tl -> in_tree k (Two_t tl pm tr)
+      | InTwoRightTree :
+          forall k tl pm tr,
+            in_tree k tr -> in_tree k (Two_t tl pm tr)
+      | InTwoNode :
+          forall k tl km vm tr,
+            k ~= km -> in_tree k (Two_t tl (km,vm) tr)
+      | InThreeLeftTree :
+          forall k tl pl tm pr tr,
+            in_tree k tl -> in_tree k (Three_t tl pl tm pr tr)
+      | InThreeMiddleTree :
+          forall k tl pl tm pr tr,
+            in_tree k tm -> in_tree k (Three_t tl pl tm pr tr)
+      | InThreeRightTree :
+          forall k tl pl tm pr tr,
+            in_tree k tr -> in_tree k (Three_t tl pl tm pr tr)
+      | InThreeLeftNode :
+          forall k tl kl vl tm pr tr,
+            k ~= kl -> in_tree k (Three_t tl (kl,vl) tm pr tr)
+      | InThreeRightNode :
+          forall k tl pl tm kr vr tr,
+            k ~= kr -> in_tree k (Three_t tl pl tm (kr,vr) tr).
+    Hint Constructors in_tree.
+    Definition in_two_node_lib :
+      forall tl km vm tr, in_tree km (Two_t tl (km,vm) tr).
+    Proof. intros ; eapply InTwoNode ; reflexivity. Qed.
+    Hint Resolve in_two_node_lib.
+    Definition in_three_left_node_lib :
+      forall tl kl vl tm pr tr,
+        in_tree kl (Three_t tl (kl,vl) tm pr tr).
+    Proof. intros ; eapply InThreeLeftNode ; reflexivity. Qed.
+    Hint Resolve in_three_left_node_lib.
+    Definition in_three_right_node_lib :
+      forall tl pl tm kr vr tr,
+        in_tree kr (Three_t tl pl tm (kr,vr) tr).
+    Proof. intros ; eapply InThreeRightNode ; reflexivity. Qed.
+    Hint Resolve in_three_right_node_lib.
 
     Inductive tree_iwf : ext_top_bot K -> ext_top_bot K -> N -> tree K V -> Prop :=
       | NullWF :
@@ -56,7 +99,74 @@ Module TwoThreeTreesWF.
            -> tm_upper_bound < inject kr < tr_lower_bound
            -> tree_iwf tl_lower_bound tr_upper_bound (t_height+1)
                        (Three_t tl (kl,vl) tm (kr,vr) tr).
+    Hint Constructors tree_iwf.
 
+    Inductive in_context : K -> context K V -> Prop :=
+      | InTwoLeftHoleContext :
+          forall k pm tr c,
+            in_context k c -> in_context k (TwoLeftHole_c pm tr c)
+      | InTwoLeftHoleTree :
+          forall k pm tr c,
+            in_tree k tr -> in_context k (TwoLeftHole_c pm tr c)
+      | InTwoLeftHoleNode :
+          forall k km vm tr c,
+            k ~= km -> in_context k (TwoLeftHole_c (km,vm) tr c)
+      | InTwoRightHoleContext :
+          forall k tl pm c,
+            in_context k c -> in_context k (TwoRightHole_c tl pm c)
+      | InTwoRightHoleTree :
+          forall k tl pm c,
+            in_tree k tl -> in_context k (TwoRightHole_c tl pm c)
+      | InTwoRightHoleNode :
+          forall k tl km vm c,
+            k ~= km -> in_context k (TwoRightHole_c tl (km,vm) c)
+      | InThreeLeftHoleContext :
+          forall k pl tm pr tr c,
+            in_context k c -> in_context k (ThreeLeftHole_c pl tm pr tr c)
+      | InThreeLeftHoleMiddleTree :
+          forall k pl tm pr tr c,
+            in_tree k tm -> in_context k (ThreeLeftHole_c pl tm pr tr c)
+      | InThreeLeftHoleRightTree :
+          forall k pl tm pr tr c,
+            in_tree k tr -> in_context k (ThreeLeftHole_c pl tm pr tr c)
+      | InThreeLeftHoleLeftNode :
+          forall k kl vl tm pr tr c,
+            k ~= kl -> in_context k (ThreeLeftHole_c (kl,vl) tm pr tr c)
+      | InThreeLeftHoleRightNode :
+          forall k pl tm kr vr tr c,
+            k ~= kr -> in_context k (ThreeLeftHole_c pl tm (kr,vr) tr c)
+      | InThreeMiddleHoleContext :
+          forall k tl pl pr tr c,
+            in_context k c -> in_context k (ThreeMiddleHole_c tl pl pr tr c)
+      | InThreeMiddleHoleLeftTree :
+          forall k tl pl pr tr c,
+            in_tree k tl -> in_context k (ThreeMiddleHole_c tl pl pr tr c)
+      | InThreeMiddleHoleRightTree :
+          forall k tl pl pr tr c,
+            in_tree k tr -> in_context k (ThreeMiddleHole_c tl pl pr tr c)
+      | InThreeMiddleHoleLeftNode :
+          forall k tl kl vl pr tr c,
+            k ~= kl -> in_context k (ThreeMiddleHole_c tl (kl,vl) pr tr c)
+      | InThreeMiddleHoleRightNode :
+          forall k tl pl kr vr tr c,
+            k ~= kr -> in_context k (ThreeMiddleHole_c tl pl (kr,vr) tr c)
+      | InThreeRightHoleContext :
+          forall k tl pl tm pr c,
+            in_context k c -> in_context k (ThreeRightHole_c tl pl tm pr c)
+      | InThreeRightHoleLeftTree :
+          forall k tl pl tm pr c,
+            in_tree k tl -> in_context k (ThreeRightHole_c tl pl tm pr c)
+      | InThreeRightHoleMiddleTree :
+          forall k tl pl tm pr c,
+            in_tree k tm -> in_context k (ThreeRightHole_c tl pl tm pr c)
+      | InThreeRightHoleLeftNode :
+          forall k tl kl vl tm pr c,
+            k ~= kl -> in_context k (ThreeRightHole_c tl (kl,vl) tm pr c)
+      | InThreeRightHoleRightNode :
+          forall k tl pl tm kr vr c,
+            k ~= kr -> in_context k (ThreeRightHole_c tl pl tm (kr,vr) c).
+    Hint Constructors in_context.
+            
     Inductive context_iwf
         : ext_top_bot K -> ext_top_bot K -> N (* bounds and height of hole *)
        -> ext_top_bot K -> ext_top_bot K -> N (* bounds and height when filled *)
@@ -142,13 +252,56 @@ Module TwoThreeTreesWF.
            -> context_iwf h_lower_bound h_upper_bound h_height
                           c_lower_bound c_upper_bound c_height
                           (ThreeRightHole_c tl (kl,vl) tm (kr,vr) c).
+    Hint Constructors context_iwf.
+
+  Inductive in_location : K -> location K V -> Prop :=
+    | InLocTwoHoleContext :
+        forall k tl tr c,
+          in_context k c -> in_location k (TwoHole_l tl tr c)
+    | InLocTwoHoleLeftTree :
+        forall k tl tr c,
+          in_tree k tl -> in_location k (TwoHole_l tl tr c)
+    | InLocTwoHoleRightTree :
+        forall k tl tr c,
+          in_tree k tr -> in_location k (TwoHole_l tl tr c)
+    | InLocThreeLeftHoleContext :
+        forall k tl tm pr tr c,
+          in_context k c -> in_location k (ThreeLeftHole_l tl tm pr tr c)
+    | InLocThreeLeftHoleLeftTree :
+        forall k tl tm pr tr c,
+          in_tree k tl -> in_location k (ThreeLeftHole_l tl tm pr tr c)
+    | InLocThreeLeftHoleMiddleTree :
+        forall k tl tm pr tr c,
+          in_tree k tm -> in_location k (ThreeLeftHole_l tl tm pr tr c)
+    | InLocThreeLeftHoleRightTree :
+        forall k tl tm pr tr c,
+          in_tree k tr -> in_location k (ThreeLeftHole_l tl tm pr tr c)
+    | InLocThreeLeftHoleNode :
+        forall k tl tm kr vr tr c,
+          k ~= kr -> in_location k (ThreeLeftHole_l tl tm (kr,vr) tr c)
+    | InLocThreeRightHoleContext :
+        forall k tl pl tm tr c,
+          in_context k c -> in_location k (ThreeRightHole_l tl pl tm tr c)
+    | InLocThreeRightHoleLeftTree :
+        forall k tl pl tm tr c,
+          in_tree k tl -> in_location k (ThreeRightHole_l tl pl tm tr c)
+    | InLocThreeRightHoleMiddleTree :
+        forall k tl pl tm tr c,
+          in_tree k tm -> in_location k (ThreeRightHole_l tl pl tm tr c)
+    | InLocThreeRightHoleRightTree :
+        forall k tl pl tm tr c,
+          in_tree k tm -> in_location k (ThreeRightHole_l tl pl tm tr c)
+    | InLocThreeRightHoleNode :
+        forall k tl kl vl tm tr c,
+          k ~= kl -> in_location k (ThreeRightHole_l tl (kl,vl) tm tr c).
+  Hint Constructors in_location.
 
   Inductive location_iwf 
-      : ext_top_bot K -> ext_top_bot K -> N (* bounds and height of hole *)
+      : ext_top_bot K -> ext_top_bot K (* bounds of hole *)
      -> ext_top_bot K -> ext_top_bot K -> N (* bounds and height when filled *)
      -> location K V
      -> Prop :=
-    | TwoHoleWF :
+    | LocTwoHoleWF :
         forall
           t_height
           tl tl_lower_bound tl_upper_bound
@@ -158,9 +311,44 @@ Module TwoThreeTreesWF.
          -> tree_iwf tr_lower_bound tr_upper_bound t_height tr
          -> context_iwf tl_lower_bound tr_upper_bound (t_height+1)
                         c_lower_bound c_upper_bound c_height c
-         -> location_iwf tl_upper_bound tr_lower_bound t_height
+         -> location_iwf tl_upper_bound tr_lower_bound
                          c_lower_bound c_upper_bound c_height
-                         (TwoHole_l tl tr c).
+                         (TwoHole_l tl tr c)
+    | LocThreeLeftHoleWF :
+        forall
+          t_height
+          tl tl_lower_bound tl_upper_bound
+          tm tm_lower_bound tm_upper_bound
+          tr tr_lower_bound tr_upper_bound
+          c c_lower_bound c_upper_bound c_height
+          kr vr,
+            tree_iwf tl_lower_bound tl_upper_bound t_height tl
+         -> tree_iwf tm_lower_bound tm_upper_bound t_height tm
+         -> tree_iwf tr_lower_bound tr_upper_bound t_height tr
+         -> tm_upper_bound < inject kr < tr_lower_bound
+         -> context_iwf tl_lower_bound tr_upper_bound (t_height+1)
+                        c_lower_bound c_upper_bound c_height c
+         -> location_iwf tl_upper_bound tm_lower_bound
+                         c_lower_bound c_upper_bound c_height
+                         (ThreeLeftHole_l tl tm (kr,vr) tr c)
+    | LocThreeRightHoleWF :
+        forall
+          t_height
+          tl tl_lower_bound tl_upper_bound
+          tm tm_lower_bound tm_upper_bound
+          tr tr_lower_bound tr_upper_bound
+          c c_lower_bound c_upper_bound c_height
+          kl vl,
+            tree_iwf tl_lower_bound tl_upper_bound t_height tl
+         -> tree_iwf tm_lower_bound tm_upper_bound t_height tm
+         -> tree_iwf tr_lower_bound tr_upper_bound t_height tr
+         -> tl_upper_bound < inject kl < tm_lower_bound
+         -> context_iwf tl_lower_bound tr_upper_bound (t_height+1)
+                        c_lower_bound c_upper_bound c_height c
+         -> location_iwf tm_upper_bound tr_lower_bound
+                         c_lower_bound c_upper_bound c_height
+                         (ThreeRightHole_l tl (kl,vl) tm  tr c).
+  Hint Constructors location_iwf.
             
   Global Instance tree_WellFormed : WellFormed (tree K V) :=
     { wf :=
@@ -171,6 +359,8 @@ Module TwoThreeTreesWF.
 
   Local Ltac mysimp :=
   match goal with
+   | [ |- forall  _,  _ ] => intros
+   | [ |- _ /\ _ ] => constructor
    | [ |- tree_iwf _ _ _ (Two_t _ _ _) ] => econstructor
    | [ |- tree_iwf _ _ _ (Three_t _ _ _ _ _) ] => econstructor
    | [ |- context_iwf _ _ _ _ _ _ Top_c ] => econstructor
@@ -179,11 +369,34 @@ Module TwoThreeTreesWF.
    | [ |- context_iwf _ _ _ _ _ _ (ThreeLeftHole_c _ _ _ _ _) ] => econstructor
    | [ |- context_iwf _ _ _ _ _ _ (ThreeMiddleHole_c _ _ _ _ _) ] => econstructor
    | [ |- context_iwf _ _ _ _ _ _ (ThreeRightHole_c _ _ _ _ _) ] => econstructor
+   | [ |- location_iwf _ _ _ _ _ (TwoHole_l _ _ _) ] => econstructor
+   | [ |- location_iwf _ _ _ _ _ (ThreeLeftHole_l _ _ _ _ _) ] => econstructor
+   | [ |- location_iwf _ _ _ _ _ (ThreeRightHole_l _ _ _ _ _) ] => econstructor
+   | [ H : _ = _ <=>! _ |- _ ] => symmetry in H
+   | [ H : _ <=>! _ = Eq |- _ ] => apply ord_dec_correct_eqv in H
+   | [ H : _ <=>! _ = Lt |- _ ] => apply ord_dec_correct_lt in H
+   | [ H : _ <=>! _ = Gt |- _ ] => apply ord_dec_correct_gt in H
+   | [ H : ?a < ?b < ?c |- ?a < ?b ] => apply H
+   | [ H : ?a < ?b < ?c |- ?b < ?c ] => apply H
+   | [ H : in_tree _ Null_t |- _ ] => inversion H
+   | [ H : in_tree _ (Two_t _ _ _) |- _ ] => inversion H ; subst ; clear H
+   | [ H : in_tree _ (Three_t _ _ _ _ _) |- _ ] => inversion H ; subst ; clear H
    | [ H : tree_iwf _ _ _ Null_t |- _ ] =>
        inversion H ; subst ; clear H
    | [ H : tree_iwf _ _ _ (Two_t _ _ _) |- _ ] =>
        inversion H ; subst ; clear H
    | [ H : tree_iwf _ _ _ (Three_t _ _ _ _ _) |- _ ] =>
+       inversion H ; subst ; clear H
+   | [ H : in_context _ Top_c |- _ ] => inversion H
+   | [ H : in_context _ (TwoLeftHole_c _ _ _) |- _ ] =>
+       inversion H ; subst ; clear H
+   | [ H : in_context _ (TwoRightHole_c _ _ _) |- _ ] =>
+       inversion H ; subst ; clear H
+   | [ H : in_context _ (ThreeLeftHole_c _ _ _ _ _) |- _ ] =>
+       inversion H ; subst ; clear H
+   | [ H : in_context _ (ThreeMiddleHole_c _ _ _ _ _) |- _ ] =>
+       inversion H ; subst ; clear H
+   | [ H : in_context _ (ThreeRightHole_c _ _ _ _ _) |- _ ] =>
        inversion H ; subst ; clear H
    | [ H : context_iwf _ _ _ _ _ _ Top_c |- _ ] =>
        inversion H ; subst ; clear H
@@ -197,14 +410,57 @@ Module TwoThreeTreesWF.
        inversion H ; subst ; clear H
    | [ H : context_iwf _ _ _ _ _ _ (ThreeRightHole_c _ _ _ _ _) |- _ ] =>
        inversion H ; subst ; clear H
-   | [ H : location_iwf _ _ _ _ _ _ (TwoHole_l _ _ _) |- _ ] =>
+   | [ H : in_location _ (TwoHole_l _ _ _) |- _ ] =>
        inversion H ; subst ; clear H
-   | [ H : location_iwf _ _ _ _ _ _ (ThreeLeftHole_l _ _ _ _ _) |- _ ] =>
+   | [ H : in_location _ (ThreeLeftHole_l _ _ _ _ _) |- _ ] =>
        inversion H ; subst ; clear H
-   | [ H : location_iwf _ _ _ _ _ _ (ThreeRightHole_l _ _ _ _ _) |- _ ] =>
+   | [ H : in_location _ (ThreeRightHole_l _ _ _ _ _) |- _ ] =>
        inversion H ; subst ; clear H
+   | [ H : location_iwf _ _ _ _ _ (TwoHole_l _ _ _) |- _ ] =>
+       inversion H ; subst ; clear H
+   | [ H : location_iwf _ _ _ _ _ (ThreeLeftHole_l _ _ _ _ _) |- _ ] =>
+       inversion H ; subst ; clear H
+   | [ H : location_iwf _ _ _ _ _ (ThreeRightHole_l _ _ _ _ _) |- _ ] =>
+       inversion H ; subst ; clear H
+   | [ H1 : ?X, H2 : ?X -> ?Y |- ?Y ] => apply (H2 H1)
+   | [ |- context [match ?x <=>! ?y with _ => _ end] ] =>
+       remember (x <=>! y) as cmp ; destruct cmp
+   | [ H : forall c' k,
+             (@?X c' k) c' k
+          /\ (@?Y c' k) c' k
+     |- _ ] =>
+       let c' := fresh "c'" in
+       let k := fresh "k" in
+       let H1 := fresh in
+       let H2 := fresh in
+       assert (forall c' k, X c' k) as H1;
+         [ intros c' k ; apply (proj1 (H c' k)) | idtac ] ;
+       assert (forall c' k, Y c' k) as H2;
+         [ intros c' k ; apply (proj2 (H c' k)) | idtac ] ;
+       clear H ; simpl in H1 ; simpl in H2
+   | [ |- context [ let (_,_) := ?p in _ ] ] => destruct p
+   | [ H1 : ?x ~= ?z, H2 : ?y ~= ?z, H3 : ?x /~= ?y |- _ ] =>
+       exfalso ; apply H3 ; transitivity z ; [ apply H1 | symmetry ; apply H2 ]
    | _ => eauto
   end.
+
+  Lemma zip_in :
+    forall (c:context K V) (t:tree K V) (k:K),
+      (in_context k c -> in_tree k (zip t c))
+   /\ (in_tree k t -> in_tree k (zip t c)).
+  Proof.
+    intros c ; induction c ; repeat mysimp.
+  Qed.
+  Lemma zip_in_context :
+    forall (c:context K V) (t:tree K V) (k:K),
+      in_context k c -> in_tree k (zip t c).
+  Proof. apply zip_in. Qed.
+  Hint Resolve zip_in_context.
+  Lemma zip_in_tree :
+    forall (c:context K V) (t:tree K V) (k:K),
+      in_tree k t -> in_tree k (zip t c).
+  Proof. apply zip_in. Qed.
+  Hint Resolve zip_in_tree.
 
   Lemma zip_wf :
     forall 
@@ -216,10 +472,27 @@ Module TwoThreeTreesWF.
                     c_lower_bound c_upper_bound c_height c
      -> tree_iwf c_lower_bound c_upper_bound c_height (zip t c).
   Proof.
-    intros c.
-    induction c ; simpl ; intros ; repeat mysimp ; eapply IHc ; repeat mysimp.
+    intros c ; induction c ; repeat mysimp ; eapply IHc ; repeat mysimp.
   Qed.
   Hint Resolve zip_wf.
+
+  Lemma fuse_in :
+    forall (c1:context K V) (c2:context K V) k,
+      (in_context k c1 -> in_context k (fuse c1 c2))
+   /\ (in_context k c2 -> in_context k (fuse c1 c2)).
+  Proof.
+    intros c ; induction c ; simpl ; repeat mysimp.
+  Qed.
+  Lemma fuse_in_context1 :
+    forall (c1:context K V) (c2:context K V) k,
+      in_context k c1 -> in_context k (fuse c1 c2).
+  Proof. apply fuse_in. Qed.
+  Hint Resolve fuse_in_context1.
+  Lemma fuse_in_context2 :
+    forall (c1:context K V) (c2:context K V) k,
+      in_context k c2 -> in_context k (fuse c1 c2).
+  Proof. apply fuse_in. Qed.
+  Hint Resolve fuse_in_context2.
 
   Lemma fuse_wf :
     forall
@@ -234,78 +507,109 @@ Module TwoThreeTreesWF.
      -> context_iwf c1h_lower_bound c1h_upper_bound c1h_height
                     c2_lower_bound c2_upper_bound c2_height (fuse c1 c2).
   Proof.
-    intros c1.
-    induction c1 ; simpl ; intros ; repeat mysimp.
+    intros c1 ; induction c1 ; simpl ; repeat mysimp.
   Qed.
   Hint Resolve fuse_wf.
+
+  Lemma fill_location_in :
+    forall (l:location K V) (k:K) (v:V),
+      (in_tree k (fill_location (k,v) l))
+   /\ (forall k', in_location k' l -> in_tree k' (fill_location (k,v) l)).
+  Proof.
+    intros l ; induction l ; simpl ; repeat mysimp.
+  Qed.
+  Lemma fill_location_in_filled :
+    forall (l:location K V) (k:K) (v:V),
+      in_tree k (fill_location (k,v) l).
+  Proof. intros ; apply (proj1 (fill_location_in _ _ _)). Qed.
+  Hint Resolve fill_location_in_filled.
+  Lemma fill_location_in_tree :
+    forall (l:location K V) (k:K) (v:V) (k':K),
+      in_location k' l -> in_tree k' (fill_location (k,v) l).
+  Proof. intros * * * * H ; apply (proj2 (fill_location_in _ _ _) _ H). Qed.
+  Hint Resolve fill_location_in_tree.
 
   Lemma fill_location_wf :
     forall
       (l:location K V) (k:K) (v:V)
-      h_lower_bound h_upper_bound h_height
+      h_lower_bound h_upper_bound
       c_lower_bound c_upper_bound c_height,
         h_lower_bound < inject k < h_upper_bound
-     -> location_iwf h_lower_bound h_upper_bound h_height
+     -> location_iwf h_lower_bound h_upper_bound
                      c_lower_bound c_upper_bound c_height l
      -> tree_iwf c_lower_bound c_upper_bound c_height (fill_location (k,v) l).
   Proof.
-    intros l.
-    induction l ; intros ; repeat mysimp.
-    eapply zip_wf ; repeat mysimp.
+    intros l ; induction l ; intros ; repeat mysimp ; eapply zip_wf ; repeat mysimp.
   Qed.
   Hint Resolve fill_location_wf.
+
+  Lemma locate_in :
+    forall (t:tree K V) (k:K) (c:context K V),
+      match locate k t c with
+      | inl c' =>
+          forall k',
+            (in_tree k' t -> in_context k' c')
+         /\ (in_context k' c -> in_context k' c')
+      | inr ((k',_),l) =>
+          k ~= k'
+       /\ (forall k'', k /~= k'' ->
+             (in_tree k'' t -> in_location k'' l)
+          /\ (in_context k'' c -> in_location k'' l))
+      end.
+  Proof.
+    intros t ; induction t ; intros ; simpl ; repeat mysimp ; eauto.
+    exfalso ; apply H ; transitivity k0 ; [ apply Heqcmp | symmetry ; apply H3 ].
+
+
+
+    
+    remember (k <=>! km) as cmp ; destruct cmp.
+    mysimp.
+    destruct p ; simpl in *.
+    constructor ; auto.
+    intros.
+    constructor ; intros.
+    eapply IHt2.
+    
+    unfold fst in * ; simpl in *.
+    compute.
+    split.
+    remember (k <=>! fst p) as cmp ; destruct cmp.
+    constructor.
+    eapply IHt2.
 
   Lemma locate_wf :
     forall
       (t:tree K V) (k:K) (c:context K V)
       t_lower_bound t_upper_bound t_height
       c_lower_bound c_upper_bound c_height,
-        t_lower_bound < inject k < t_upper_bound
-     -> tree_iwf t_lower_bound t_upper_bound t_height t
+        tree_iwf t_lower_bound t_upper_bound t_height t
      -> context_iwf t_lower_bound t_upper_bound t_height
                     c_lower_bound c_upper_bound c_height c
      -> exists h_lower_bound h_upper_bound,
-          h_lower_bound < inject k < h_upper_bound
-       /\ match locate k t c with
+          match locate k t c with
           | inl c =>
               context_iwf h_lower_bound h_upper_bound 0
                           c_lower_bound c_upper_bound c_height c
-          | inr ((k,v),l) =>
-              exists h_height,
-                location_iwf h_lower_bound h_upper_bound h_height
-                             c_lower_bound c_upper_bound c_height l
+          | inr ((_,_),l) =>
+              location_iwf h_lower_bound h_upper_bound
+                           c_lower_bound c_upper_bound c_height l
           end.
   Proof.
-    intros t.
-    induction t ; intros ; simpl ; repeat mysimp.
-    simpl.
-    remember (k <=>! km) as cmp ; destruct cmp.
+    intros t ; induction t ; intros ; simpl ; repeat mysimp.
+  Qed.
 
-    symmetry in Heqcmp.
-    eapply ord_dec_correct_eqv in Heqcmp.
-    rewrite Heqcmp in H.
-    rewrite H0 in * ; clear H0 ; clear Heqcmp.
-
-    exists tl_upper_bound.
-    exists tr_lower_bound.
-    split.
-    auto.
-    exists t_height0.
-    econstructor.
-    eapply H8.
-    eapply H9.
-    eapply H1.
-
-    assert (lt k km). admit.
-    assert (t_lower_bound < inject km < tr_lower_bound).
-      split.
-      transitivity (inject k).
-
-    eapply IHt1. 
-    eapply H.
-    eapply H8.
-
-    exists tl_upper_bound.
-
+  Lemma locate_greatest_wf :
+    forall
+      (t:tree K V) (c:context K V)
+      t_lower_bound t_upper_bound t_height
+      c_lower_bound c_upper_bound c_height,
+        tree_iwf t_lower_bound t_upper_bound t_height
+     -> context_iwf t_lower_bound t_upper_bound t_height
+                    c_lower_bound c_upper_bound c_height c
+     -> exists h_lower_bound h_upper_bound,
+          match locate_greatest t c with
+          | None => t = Null_t
+          | Some l
   
 End TwoThreeTreesWF.
